proof/equivHybrid.ec
@@ -28,6 +28,142 @@ proof.
   inline {1} Dkc.Dkc.get_challenge.
   inline {1} Dkc.Dkc.initialize.
   inline {1} Dkc.Dkc.encrypt.
+  inline {1} AdvGate.Adv(Adv).gen_queries.
+  inline {1} AdvGate.Adv(Adv).get_challenge.
+  inline {1} AdvGate.Adv(Adv).compute0.
+  inline {1} AdvGate.Adv(Adv).gen_queries0.
+  inline {2} Dkc.Dkc.preInit.
+  inline {2} Dkc.Dkc.get_challenge.
+  inline {2} Dkc.Dkc.initialize.
+  inline {2} Dkc.Dkc.encrypt.
+  inline {2} AdvGate.Adv(Adv).gen_queries.
+  inline {2} AdvGate.Adv(Adv).get_challenge.
+  inline {2} AdvGate.Adv(Adv).compute1.
+  inline {2} AdvGate.Adv(Adv).gen_queries1.
+ 
+  swap [7..9] -6.
+
+  app 3 3 : (
+    AdvGate.Adv.c{1} = AdvGate.Adv.c{2} /\
+    AdvGate.Adv.fc{1} = AdvGate.Adv.fc{2} /\
+    AdvGate.Adv.xc{1} = AdvGate.Adv.xc{2} /\
+    query{1} = query{2} /\
+    AdvGate.Adv.l{1}=0 /\
+    Dkc.Dkc.b{1} = false /\
+    AdvGate.Adv.l{2}=1 /\
+    Dkc.Dkc.b{2} = true
+  ).
+wp. call true (res{1}=res{2}).
+admit.
+rnd.
+skip.
+simplify.
+intros &1 &2 h.
+intros x hypx. split. trivial.
+intros hypx2 hypx3.
+intros L R hypLR.
+simplify.
+trivial.
+[admit|rnd;skip;trivial]|]. (* Call adv gen_queries *)
+
+  case (Gate.eval (fst (fst query{2})) (snd (fst query{2})) = Gate.eval (fst (snd query{2})) (snd (snd query{2}))). (*good*)
+
+  rcondt {1} 9;[intros &m;wp;rnd;wp;rnd;skip;trivial|]. (*good*)
+  rcondf {1} 11;[admit|]. (* l condition *)
+  rcondt {1} 10;[admit|]. (* l condition *)
+  rcondt {1} 17;[admit|]. (* While *)
+  rcondt {1} 24;[admit|]. (* While *)
+  rcondf {1} 31;[admit|]. (* While *)
+  rcondt {1} 33;[admit|]. (* good *)
+  rcondf {1} 34;[admit|]. (* l *)
+  rcondt {1} 33;[admit|]. (* l *)
+
+  rcondt {2} 9;[intros &m;wp;rnd;wp;rnd;skip;trivial|]. (*good*)
+  rcondf {2} 10;[admit|]. (* l condition *)
+  rcondt {2} 10;[admit|]. (* l condition *)
+  rcondt {2} 18;[admit|]. (* While *)
+  rcondt {2} 25;[admit|]. (* While *)
+  rcondf {2} 32;[admit|]. (* While *)
+  rcondt {2} 34;[admit|]. (* good *)
+  rcondf {2} 34;[admit|]. (* l *)
+  rcondt {2} 34;[admit|]. (* l *)
+
+  wp.
+  call (answer{1}=answer{2}) (res{1} = res{2});[admit|].
+  wp.
+  swap{1} [5..6] -3. (*rewrite tau*)
+  swap{1} 9 -5. (*rewrite tau*)
+  swap{1} 10 -5. (*t*)
+  swap{1} 38 -32. (*keyntau*)
+
+  swap{2} 10 -9. (*t*)
+  swap{1} [6..7] -2. (*rewrite tau*)
+  swap{1} 10 -5. (*rewrite tau*)
+  swap{2} 39 -30. (*key_nt_ntau*)
+  swap{2} 39 -25. (*keyntau*)
+  swap{1} 38 -25. (*keyntau*)
+  swap{1} 10 -8. (*t*)
+  swap{2} 11 -10. (*t*)
+
+  case (
+(Gate.eval AdvGate.Adv.fc{1} AdvGate.Adv.xc{1}=Gate.eval AdvGate.Adv.fc{1} (!(fst AdvGate.Adv.xc{1}), (snd AdvGate.Adv.xc{1}))) /\
+(Gate.eval AdvGate.Adv.fc{2} AdvGate.Adv.xc{2}=Gate.eval AdvGate.Adv.fc{2} (!(fst AdvGate.Adv.xc{2}), (snd AdvGate.Adv.xc{2})))
+).
+  rcondt{1} 37;[admit|].
+  rcondt{1} 38;[admit|].
+  rcondt{2} 39;[admit|].
+  wp.
+
+  (*BEGIN CLEAN DKC*)
+  (*LOOP 2*)
+  (rcondt {1} 28;[admit|]). (* Dkc used *)
+  (rcondt {1} 29;[admit|]). (* Dkc not reusing *)
+  (rcondt {1} 30;[admit|]). (* Dkc not reusing *) (*TODO: FALSE*)
+  (rcondt {1} 31;[admit|]). (* Dkc not reusing *)
+  (rcondt {2} 30;[admit|]). (* Dkc used *)
+  (rcondt {2} 31;[admit|]). (* Dkc not reusing *)
+  (rcondt {2} 32;[admit|]). (* Dkc not reusing *)
+  (rcondt {2} 33;[admit|]). (* Dkc not reusing *)
+  (*LOOP 1*)
+  (rcondt {1} 21;[admit|]). (* Dkc used *)
+  (rcondt {1} 22;[admit|]). (* Dkc not reusing *)
+  (rcondt {1} 23;[admit|]). (* Dkc not reusing *)
+  (rcondt {1} 24;[admit|]). (* Dkc not reusing *)
+  (rcondt {2} 23;[admit|]). (* Dkc used *)
+  (rcondt {2} 24;[admit|]). (* Dkc not reusing *)
+  (rcondt {2} 25;[admit|]). (* Dkc not reusing *)
+  (rcondt {2} 26;[admit|]). (* Dkc not reusing *)
+  (*END CLEAN DKC*)
+
+  wp.
+
+  rnd.
+  rnd.
+  swap{2} 37 -34.
+
+OLD STUFF :
+
+
+
+
+
+
+
+
+
+
+  rcondt {1} 11;[intros &m;wp;rnd;wp;rnd;rnd;skip;trivial|].
+  rcondt {2} 11;[intros &m;wp;rnd;wp;rnd;rnd;skip;trivial|].
+
+
+[intros &m;*(wp;try rnd;wp;try (call true true;admit);wp;try (skip;trivial))|]);
+
+
+
+  inline {1} Dkc.Dkc.preInit.
+  inline {1} Dkc.Dkc.get_challenge.
+  inline {1} Dkc.Dkc.initialize.
+  inline {1} Dkc.Dkc.encrypt.
   inline {1} AdvGate.Adv.gen_queries.
   inline {1} AdvGate.Adv.get_challenge.
   rcondt {1} 8;[admit|].
